first try at phoas sysf with sub

Types/SysFHOAS/Denote.lean
@@ -2,7 +2,7 @@ import Types.SysFHOAS.Stx
 
 namespace SysFPHOAS
 
-universe u
+universe u v w
 
 @[simp]
 def Type'.denote : Type' (Sort u) → Sort (u + 1)
@@ -10,13 +10,20 @@ def Type'.denote : Type' (Sort u) → Sort (u + 1)
   | .arr t1 t2 => Type'.denote t1 → Type'.denote t2
   | .all f => (T : Sort u) → Type'.denote (f T)
 
-@[simp]
-def Term'.denote {ty : Type' (Sort u)} : Term' (Type'.denote) ty → ty.denote
+def Term'.denote {n} {ty : Type'.higher n (Sort u)} : Term' (fun n => Type'.denote ∘ Type'.compress) n ty → (Type'.compress ty).denote
   | .var v => v
-  | .app t1 t2 => (Term'.denote t1) (Term'.denote t2)
+  | .app t1 t2 => by
+    have a := (Term'.denote t1)
+    have b := (Term'.denote t2)
+    unfold Type'.compress at a
+    dsimp at a
+    sorry
   | .lam f => fun x => Term'.denote (f x)
-  | @Term'.tapp _ _ _f term1 t => (Term'.denote term1) t
-  | @Term'.tlam _ _ f g => fun x => Term'.denote (g x)
+  | @Term'.tapp _ _ _f term1 t =>
+    (Term'.denote term1) t
+  | @Term'.tlam _ _ f g => 
+    sorry
+    fun x => Term'.denote (g x)
 
 def same {ty : Ty} (t1 t2 : Term ty) : Prop :=
   Term'.denote t1 = Term'.denote t2
