Types/Ex2.lean
@@ -1,0 +1,72 @@
+import Types.SysFHOAS.Show
+import Types.SysFHOAS.Denote
+
+namespace SysFPHOAS
+
+universe u
+
+open Term' (var)
+
+namespace Ex1
+
+def a.t : Ty := .arr
+  (.all fun α ↦ .var α) (.all fun β => .var β)
+
+def a.e : Term a.t :=
+  .lam fun x => .tlam fun β => .tapp (.var x) β
+
+-- This cant exist because α is not a unit type
+
+-- TODO: C , A₃ must be False, i.e. ∀ α, α
+-- TODO: D , A₄ could be the constant false function,
+--           but this cannot exist in the given context as (x α) isnt a type.
+
+end Ex1
+
+section Ex2
+
+-- The eliminator for the Unit type is simply id, so its encoding is 
+
+def unit : Ty := .all fun α => .arr (.var α) (.var α)
+def unit.i : Term unit := .tlam fun _ => .lam fun v => .var v
+
+def emp : Ty := .all fun α => .var α
+def emp.e : Term (.all fun x => .arr emp (.var x)) :=
+  .tlam fun β => .lam fun e => .tapp (.var e) β
+
+variable (X : Ty) {rep : Type u} {rep2 : Type' rep → Type u}
+
+def tree : Ty := .all fun α => 
+  .arr (.var α) <| .arr
+    (.arr (.var α) <| .arr X <| .arr (.var α) (.var α))
+    (.var α)
+def tree.leaf : Term (tree X) := 
+  .tlam fun _ => .lam fun lf => .lam fun _ => .var lf
+def tree.node : Term (.arr (tree X) <| .arr X <| .arr (tree X) (tree X)) := 
+  .lam fun l => .lam fun c => .lam fun r =>
+    .tlam fun β =>
+      .lam fun bot =>
+        .lam fun main =>
+          have l : Term' _ (Type'.var β) :=
+            var l |>.tapp β |>.app (.var bot) |>.app (.var main)
+          have r : Term' _ (Type'.var β) :=
+            var r |>.tapp β |>.app (.var bot) |>.app (.var main)
+          var main |>.app l |>.app (.var c) |>.app r
+
+def prod (A B : rep) : Type' rep :=
+  .all fun s => .arr (.arr (.var A) (.arr (.var B) (.var s))) (.var s)
+
+def prod.fst (A B : rep) : Term' rep2 (.arr (prod A B) (.var A)) :=
+  .lam fun ab =>
+    var ab |>.tapp A |>.app
+      (.lam fun v => .lam fun _ => .var v)
+
+def prod.snd (A B : rep) : Term' rep2 (.arr (prod A B) (.var B)) :=
+  .lam fun ab =>
+    var ab |>.tapp B |>.app
+      (.lam fun _ => .lam fun v => .var v)
+
+end Ex2
+
+end SysFPHOAS
+
