Types/SysFHOAS/Stx.lean
@@ -8,15 +8,54 @@ inductive Type' (rep : Type u) : Type u where
   | arr : Type' rep → Type' rep → Type' rep
   | all : (rep → Type' rep) → Type' rep
 
+def Type'.squash {rep : Type u} : Type' (Type' rep) → Type' rep
+  | .var rep => rep
+  | .arr a b => .arr a.squash b.squash
+  | .all f => .all fun v => (f (.var v)).squash
+
+def Type'.higher (n : Nat) (rep : Type u) := n.succ.repeat Type' rep
+
+def Type'.pvar {n : Nat} {rep} (r : rep) : n.repeat Type' rep :=
+  match n with
+  | 0 => r
+  | _+1 => .var (Type'.pvar r)
+
+def Type'.compress : {n : Nat} → {rep : Type u} → Type'.higher n rep → Type' rep
+  | 0, _, v => v
+  | n+1, _, .var rep => Type'.compress rep
+  | _, _, .arr a b => .arr (Type'.compress a) (Type'.compress b)
+  | _, _, .all f => sorry
+
 def Ty : Type (u + 1) :=  {rep2 : Type u} → Type' rep2
 
-inductive Term' {T: Type v} (rep : Type' T → Type u) : Type' T →  Type (max u v) where
-  | var : ∀ {t : Type' T}, rep t → Term' rep t
-  | app :  {A B : Type' T} →  Term' rep (Type'.arr A B) → Term' rep A → Term' rep B
-  | lam : ∀ {A B : Type' T}, (rep A → Term' rep B) → Term' rep (Type'.arr A B)
-  | tapp : {f : T → Type' T}  → Term' rep (Type'.all f) → (t : T) → Term' rep (f t)
-  | tlam : {f : T → Type' T} → ((x : T) → Term' rep (f x)) → Term' rep (Type'.all f)
+declare_syntax_cat hstx_ty
+
+syntax ident : hstx_ty
+syntax "!(" term ")" : hstx_ty
+syntax "(" hstx_ty ")" : hstx_ty
+syntax hstx_ty "→" hstx_ty : hstx_ty
+syntax "∀" ident+ "." hstx_ty : hstx_ty
+
+syntax "[ht|" hstx_ty "]" : term
+
+macro_rules
+  | `([ht| $v:ident ]) => `(Type'.var $v)
+  | `([ht| !($t) ]) => `($t)
+  | `([ht| $a → $b ]) => `(Type'.arr [ht| $a] [ht| $b])
+  | `([ht| ($v) ]) => `(([ht|$v]))
+  | `([ht| ∀ $i. $v]) => `(Type'.all fun $i => ([ht|$v]))
+  | `([ht| ∀ $i $is*. $v]) => `(Type'.all fun $i => ([ht| ∀ $is*. $v]))
+
+inductive Term' {T: Type v} (rep : ∀ n, Type'.higher n T → Type u) : (n : Nat) → Type'.higher n T → Type (max u v) where
+  | var {n t} : rep n t → Term' rep n t
+  | app {n A B} : Term' rep n (Type'.arr A B) → Term' rep n A → Term' rep n B
+  | lam {n A B}: (rep n A → Term' rep n B) → Term' rep n (Type'.arr A B)
+  | tapp {n} : {f : Type'.higher n T → Type'.higher n.succ T}
+    → Term' rep n.succ (Type'.all f)
+    → (t : Type'.higher n T)
+    → Term' rep n (f t).squash
+  | tlam {n f} : ((x : _) → Term' rep n (f x)) → Term' rep n (Type'.all f)
 
 def Term (t : Ty) : Type (u + 1) :=
-  {T : Type u} → {rep : Type' T → Type u} → Term' rep t
+  {T : Type u} → {n : Nat} → {rep : ∀ n, Type'.higher n T → Type u} → Term' rep n t
 
